src/common/commons.dfy
@@ -722,10 +722,11 @@ module CommonFunctions{
         k: (AttestationData, seq<bool>),
         construct_signed_attestation_signature: (set<AttestationShare>) -> Optional<BLSSignature>, 
         rcvd_attestation_shares: map<Slot,map<(AttestationData, seq<bool>), set<AttestationShare>>>
-    ): Attestation
+    ): (aggregated_attestation: Attestation)
     requires attestation_share.data.slot in rcvd_attestation_shares.Keys
     requires k in rcvd_attestation_shares[attestation_share.data.slot]
     requires construct_signed_attestation_signature(rcvd_attestation_shares[attestation_share.data.slot][k]).isPresent()    
+    ensures aggregated_attestation.data == attestation_share.data
     {
         Attestation(
             aggregation_bits := attestation_share.aggregation_bits,
