src/proofs/common/helper_sets_lemmas.dfy
@@ -514,4 +514,5 @@ function intsetmax(s:set<int>):int
     requires S1 <= S2 && S2 <= S3
     ensures S1  <= S3
     {}
+
 }
